# Question 5: Sum linked lists

You have two numbers represented by a linked list, where each node contains a single digits. The gigits are stored in reverse order.

Example:

```
Input: 7->1->6 + 5->9->2.
That is: 617 + 295 = 912
Output: 2->1->9
```

This is actually very straight forward, but hard to write.

## Soltuion

Algorithm:

0. Initialize:

   - ListNode Dummy : Dummy.next will be our returned list
   - ListNode current: current = Dummy
   - ListNode p, q : p = l1, q = l2
   - int carry: the value when two numbers add up > 10;

1. Iterate over l1 and l2 until p and q are both null:

   - int x = p == null ? 0 : p.val;
   - int y = q == null ? 0 : q.val;
   - int sum = x + y;
   - carry = sum / 10;
   - carry.next = new ListNode(sum % 10);
   - p = p.next, q = q.next

```java
class Solution {
    public ListNode addTwoNumbers(ListNode l1, ListNode l2) {
        ListNode dummy = new ListNode(0);
        ListNode curr = dummy;  // use curr to drive down to add .next

        ListNode p = l1, q = l2;
        int carry = 0;

        while (p != null || q != null) {
            int x = (p == null) ? 0 : p.val;
            int y = (q == null) ? 0 : q.val;

            int sum = carry + x + y;
            carry = sum / 10;
            curr.next = new ListNode(sum % 10);
            curr = curr.next;
            if (p != null) p = p.next;
            if (q != null) q = q.next;
        }

        if (carry > 0) {
            curr.next = new ListNode(carry);
        }

        return dummy.next;
    }
}
```

# Question 5.5: Add two numbers (reverse order)

Example

```
6->1->7 + 2->9->5
that is 617 + 295
912
Output: 9->1->2
```

## Solution 1: We can reverse a linked list, then just use the solution in question 5.

## Reverse a Linked List

Example

```
6->1->7
becomes
7->1->6
```

## Solution 1: Iterative

```java
class Solution {
    public ListNode reverse(ListNode head) {
        ListNode prev = null;
        while (head != null) {
            ListNode next = head.next;
            head.next = prev;
            prev = head;
            head = next;
        }
        return prev;
    }
}
```

This one is tricky for one too. Let us go through the whole thing:

```
0.
head : (6,next)->(1,next)->(7,next)->null
prev : null
1. First Iteration, head != null
 next : (1,next)->(7,next)->null
 head : (6,next)->null
 prev : (6,next)->null
 head : (1,next)->(7,next)->null

2. Second Iteration, head : (1,next)->(7,next)->null != null
 next : (7,next)->null
 head : (1,next)->(6,next)->null
 prev : (1,next)->(6,next)->null
 head : (7,next)->null

3. Third Iteration, head : (7,next)->null != null
 next : null
 head : (7,next)->(1,next)->(6,next)->null
 prev : (7,next)->(1,next)->(6,next)->null
 head : null

Return prev
```

## Solution 2: Recursion

[Leetcode article](https://leetcode.com/problems/reverse-linked-list/solution/)

Algorithm:

0. Initialize node curr as head.

Boundary cases:

1. if curr is null, return.
2. if curr.next is null, that means it is the last node, make this as head because the last node will be the head of the reversed list.

Actually reversing:

3. Recursively traverse the list.
4. Set curr.next.next to curr.
5. Set curr.next to null

```java
public void reverseList(ListNode head) {
    if (head == null || head.next == null) return head;
    ListNode p = reverseList(head.next);
    head.next.next = head;
    head.next = null;
    return p;
}
```
